proofs/isabelle/SpecRest/core/Semantics_Reference.thy
@@ -19,6 +19,7 @@ definition builtins_reserved ::
   "builtins_reserved fs ps \<equiv> (\<forall>nm. is_builtin_pred nm \<longrightarrow> lookup_callee fs ps nm = None)
                               \<and> (\<forall>nm. is_builtin_const nm \<longrightarrow> lookup_callee fs ps nm = None)
                               \<and> (\<forall>nm. is_builtin_func nm \<longrightarrow> lookup_callee fs ps nm = None)
+                              \<and> (\<forall>nm. is_builtin_int_func nm \<longrightarrow> lookup_callee fs ps nm = None)
                               \<and> lookup_callee fs ps (STR ''dom'') = None
                               \<and> lookup_callee fs ps (STR ''range'') = None
                               \<and> lookup_callee fs ps (STR ''ran'') = None
@@ -182,6 +183,10 @@ and eval_forall ::
                             then (case eval fs ps fuel s st env arg of
                                     Some (VStr str) \<Rightarrow> Some (VStr (builtin_str_func nm str))
                                   | _ \<Rightarrow> None)
+                          else if is_builtin_int_func nm
+                            then (case eval fs ps fuel s st env arg of
+                                    Some (VInt n) \<Rightarrow> Some (VInt (builtin_int_func nm n))
+                                  | _ \<Rightarrow> None)
                             else None)
                      | _ \<Rightarrow> None))
            | _ \<Rightarrow> None))"
@@ -311,7 +316,8 @@ lemma eval_dom_CallF:
   assumes "lookup_callee fs ps (STR ''dom'') = None"
   shows "eval fs ps fuel s st env
            (CallF (IdentifierF (STR ''dom'') sp1) [IdentifierF rel sp2] sp) = None"
-  using assms by (simp add: is_builtin_pred_def is_builtin_func_def split: nat.splits)
+  using assms
+  by (simp add: is_builtin_pred_def is_builtin_func_def is_builtin_int_func_def split: nat.splits)
 
 lemma quant_dom_qb_names:
   "quant_dom s st k bs = Some (var, dmv) \<Longrightarrow> qb_names bs = [var]"
@@ -562,7 +568,19 @@ next
                   by (auto split: option.splits ir_value.splits)
               next
                 case False
-                thus ?thesis using Suc idc None ac Nil \<open>\<not> is_builtin_pred nm\<close> by simp
+                show ?thesis
+                proof (cases "is_builtin_int_func nm")
+                  case True
+                  have "eval fs ps fuel s st env a = eval fs ps fuel s st env2 a"
+                    using "15.IH" Suc idc None ac Nil agr \<open>\<not> is_builtin_pred nm\<close> \<open>\<not> is_builtin_func nm\<close> True
+                    by (auto simp: env_lookup_def)
+                  then show ?thesis using Suc idc None ac Nil \<open>\<not> is_builtin_pred nm\<close> \<open>\<not> is_builtin_func nm\<close> True
+                    by (auto split: option.splits ir_value.splits)
+                next
+                  case False
+                  thus ?thesis
+                    using Suc idc None ac Nil \<open>\<not> is_builtin_pred nm\<close> \<open>\<not> is_builtin_func nm\<close> by simp
+                qed
               qed
             qed
           next
@@ -1380,17 +1398,34 @@ next
           by (simp split: option.splits ir_value.splits)
       next
         case False
-        have bif: "is_builtin_func nm"
-          using "15.prems" fuel idc None aeq False
-          by (auto split: option.splits ir_value.splits if_splits)
-        obtain str where ea: "eval fs ps fuel s st env arg = Some (VStr str)"
-            and w_eq: "w = VStr (builtin_str_func nm str)"
-          using "15.prems" fuel idc None aeq False bif
-          by (auto split: option.splits ir_value.splits if_splits)
-        have ea': "eval fs ps fuel s st env (inline_calls fs ps arg) = Some (VStr str)"
-          using "15.IH" fuel idc None aeq ea False bif by (auto split: if_splits)
-        show ?thesis using inl ea' w_eq fuel idc None aeq False bif
-          by (simp split: option.splits ir_value.splits)
+        note npred = False
+        show ?thesis
+        proof (cases "is_builtin_func nm")
+          case True
+          note bif = True
+          obtain str where ea: "eval fs ps fuel s st env arg = Some (VStr str)"
+              and w_eq: "w = VStr (builtin_str_func nm str)"
+            using "15.prems" fuel idc None aeq npred bif
+            by (auto split: option.splits ir_value.splits if_splits)
+          have ea': "eval fs ps fuel s st env (inline_calls fs ps arg) = Some (VStr str)"
+            using "15.IH" fuel idc None aeq ea npred bif by (auto split: if_splits)
+          show ?thesis using inl ea' w_eq fuel idc None aeq npred bif
+            by (simp split: option.splits ir_value.splits)
+        next
+          case False
+          note nfunc = False
+          have bif: "is_builtin_int_func nm"
+            using "15.prems" fuel idc None aeq npred nfunc
+            by (auto split: option.splits ir_value.splits if_splits)
+          obtain n where ea: "eval fs ps fuel s st env arg = Some (VInt n)"
+              and w_eq: "w = VInt (builtin_int_func nm n)"
+            using "15.prems" fuel idc None aeq npred nfunc bif
+            by (auto split: option.splits ir_value.splits if_splits)
+          have ea': "eval fs ps fuel s st env (inline_calls fs ps arg) = Some (VInt n)"
+            using "15.IH" fuel idc None aeq ea npred nfunc bif by (auto split: if_splits)
+          show ?thesis using inl ea' w_eq fuel idc None aeq npred nfunc bif
+            by (simp split: option.splits ir_value.splits)
+        qed
       qed
     qed
   next
